Common/Vec.lean
@@ -978,9 +978,78 @@ def Vec.findIdxs {α : Type u_1} (p : α -> Bool) : {n : Nat} -> (v : Vec α n) 
 #guard #(0, 1, 2, 3).findIdxs (· == 0) == [0]
 #guard #(0, 1, 2, 3).findIdxs (· == 4) == []
 
--- theorem Vec.zipIdx_map {α : Type u_1} {β : Type u_2} {n : Nat} {vs : Vec α n} {k : Nat} {f : α → β} :
+@[simp]
+theorem Vec.cast_cons
+  {e1 : n = m} {e2 : Vec α n = Vec α m}
+  {x : α} {xs : Vec α n}
+  : cast (by grind) (x :: xs) = x :: cast e2 xs
+:= by
+  cases e1; simp;
+
+@[simp, grind =]
+theorem Vec.cast_get {α β : Type u} {e1 : α = β}
+  : ∀ {n : Nat} {e2 : Vec α n = Vec β n} {i : Fin n}, {v : Vec α n} -> cast e1 (v[i]) = (cast e2 v)[i]
+| 0, e2, i, .nil => by simp [getElem]; grind
+| n + 1, e2, i, .cons x xs => by
+  cases i using Fin.cases
+  case _ => cases e1; cases e2; simp
+  case _ i => cases e1; cases e2; simp
+
+-- theorem Vec.zipIxd_map {α : Type u_1} {β : Type u_2} {n : Nat} {vs : Vec α n} {k : Nat} {f : α → β} :
 --   (Vec.map f vs).zipIdx k = Vec.map (Prod.map f id) (vs.zipIdx k)
 -- := by sorry
+-- theorem Vec.list_zipWith_zipWith_list {f : α -> β -> γ} :
+--   Vec.zipWith f vs1 vs2 ≍ (Vec.from_list (List.zipWith f vs1.list vs2.list)).2
+-- := by
+--   generalize zdef : from_list (List.zipWith f vs1.list vs2.list) = z at *
+--   rcases z with ⟨z_len, zs⟩; simp at *
+--   induction vs1 generalizing z_len zs <;> cases vs2
+--   · simp at zdef; rcases zdef with ⟨e1, e2⟩; subst e1; simp at e2; subst e2; simp [Vec.zipWith]
+--   case _ n a as ih b bs =>
+--     simp [List.zipWith_cons_cons] at zdef;
+--     replace zdef := Vec.from_list_cons zdef
+--     rcases zdef with ⟨n', zs', e1, e2, e3⟩
+--     simp [Vec.zipWith]
+--     replace ih := @ih bs n' zs' e1
+--     subst e3; simp at *;
+--     subst e2; simp; congr;
+--     have lem : as.list.length = bs.list.length := by simp [Vec.length_list]
+--     have lem2 : (List.zipWith f as.list bs.list).length = as.list.length := by simp [List.length_zipWith]
+--     have lem3 : as.list.length = n := by simp [Vec.length_list]
+--     generalize kdef : Vec.zipWith f as bs = ks at *
+--     generalize k'def : List.zipWith f as.list bs.list = ks' at *
+--     have lem4 : ks.length = n := by simp
+--     have lem5 : ks'.length = n := by grind
 
+--     sorry
+
+theorem Vec.list_zipWith_iff_zipWith_list {f : α -> β -> γ} {vs1 vs2 zs : Vec _ n}:
+  Vec.zipWith f vs1 vs2 = zs ↔
+  (Vec.from_list (List.zipWith f vs1.list vs2.list)) = ⟨n, zs⟩
+:= by
+  induction vs1 <;> cases vs2
+  case _ => simp
+  case _ n a as ih b bs =>
+    simp [List.zipWith_cons_cons]
+    cases zs; case _ z zs =>
+    simp [Vec.from_list]
+    replace ih := @ih bs zs
+    simp [ih]
+    apply Iff.intro
+    simp; intro h1 h2; subst h1; simp [h2]; congr; simp [h2]; rw[h2]
+    simp; intro h1 h2; apply And.intro; sorry; sorry
+
+
+theorem Vec.mem_list {x : α} {vs : Vec α n} :
+  x ∈ vs ↔ x ∈ vs.list
+:= by
+  induction vs
+  simp; intro h; cases h
+  case _ v vs ih =>
+    simp;
+    apply Iff.intro
+    intro h; cases h; simp; apply Or.inr; apply ih.mp; assumption
+    intro h; cases h; case _ e => subst e; constructor
+    constructor; apply ih.mpr; assumption
 
 end Lilac
